src/graph_theory/to_mathlib.lean
@@ -1,5 +1,4 @@
 import combinatorics.simple_graph.basic
 
 namespace simple_graph
-def adj.symm {V : Type*} {G : simple_graph V} := G.symm
 end simple_graph
